Replace assert instruction with abort

src/lang/Configuration.v
@@ -152,18 +152,18 @@ Module Configuration.
   Qed.
 
   Inductive step: forall (e:MachineEvent.t) (tid:Ident.t) (c1 c2:t), Prop :=
-  | step_abort
+  | step_failure
       pf tid c1 lang st1 lc1 e2 st3 lc3 sc3 memory3
       (TID: IdentMap.find tid c1.(threads) = Some (existT _ lang st1, lc1))
       (STEPS: rtc (@Thread.tau_step _) (Thread.mk _ st1 lc1 c1.(sc) c1.(memory)) e2)
-      (STEP: Thread.step pf ThreadEvent.abort e2 (Thread.mk _ st3 lc3 sc3 memory3)):
-      step MachineEvent.abort tid c1 (mk (IdentMap.add tid (existT _ _ st3, lc3) c1.(threads)) sc3 memory3)
+      (STEP: Thread.step pf ThreadEvent.failure e2 (Thread.mk _ st3 lc3 sc3 memory3)):
+      step MachineEvent.failure tid c1 (mk (IdentMap.add tid (existT _ _ st3, lc3) c1.(threads)) sc3 memory3)
   | step_normal
       pf e tid c1 lang st1 lc1 e2 st3 lc3 sc3 memory3
       (TID: IdentMap.find tid c1.(threads) = Some (existT _ lang st1, lc1))
       (STEPS: rtc (@Thread.tau_step _) (Thread.mk _ st1 lc1 c1.(sc) c1.(memory)) e2)
       (STEP: Thread.step pf e e2 (Thread.mk _ st3 lc3 sc3 memory3))
-      (EVENT: e <> ThreadEvent.abort)
+      (EVENT: e <> ThreadEvent.failure)
       (CONSISTENT: Thread.consistent (Thread.mk _ st3 lc3 sc3 memory3)):
       step (ThreadEvent.get_machine_event e) tid c1 (mk (IdentMap.add tid (existT _ _ st3, lc3) c1.(threads)) sc3 memory3)
   .
@@ -181,11 +181,11 @@ Module Configuration.
 
   Definition tau_step := union (step MachineEvent.silent).
 
-  Definition steps_abort (c1: t): Prop :=
+  Definition steps_failure (c1: t): Prop :=
     exists tid c2 c3,
       <<STEPS: rtc tau_step c1 c2>> /\
-      <<ABORT: step MachineEvent.abort tid c2 c3>>.
-  Hint Unfold steps_abort.
+      <<FAILURE: step MachineEvent.failure tid c2 c3>>.
+  Hint Unfold steps_failure.
 
   Inductive has_promise (c:t): Prop :=
   | has_promise_intro
