src/invariant/PFStepCommon.v
@@ -65,11 +65,11 @@ Module PFStepCommon.
     - econs; eauto.
   Qed.
 
-  Lemma abort_step
+  Lemma failure_step
         lc1_src lc1_tgt
         (LOCAL1: sim_local lc1_src lc1_tgt)
-        (STEP_TGT: Local.abort_step lc1_tgt):
-    <<STEP_SRC: Local.abort_step lc1_src>>.
+        (STEP_TGT: Local.failure_step lc1_tgt):
+    <<STEP_SRC: Local.failure_step lc1_src>>.
   Proof.
     destruct lc1_src, lc1_tgt. inv LOCAL1. inv STEP_TGT. ss.
     subst. econs; eauto.
