src/opt/ReorderStore.v
@@ -266,11 +266,11 @@ Proof.
     + etrans; eauto. etrans; eauto.
     + left. eapply paco9_mon; [apply sim_stmts_nil|]; ss.
       etrans; eauto.
-  - (* assert fail *)
+  - (* assert failure *)
     left.
-    exploit sim_local_abort; try exact LOCAL1; eauto. i. des.
-    exploit reorder_fulfill_abort; eauto. i. des.
-    unfold Thread.steps_abort. esplits; eauto.
+    exploit sim_local_failure; try exact LOCAL1; eauto. i. des.
+    exploit reorder_fulfill_failure; eauto. i. des.
+    unfold Thread.steps_failure. esplits; eauto.
     econs 2. econs; eauto. econs. econs. ss.
 Qed.
 
@@ -296,7 +296,7 @@ Proof.
       punfold SIM. exploit SIM; try apply SC3; eauto; try refl. s. i. des.
       exploit PROMISES; eauto. i. des.
       * left.
-        unfold Thread.steps_abort in *. des.
+        unfold Thread.steps_failure in *. des.
         esplits; [|eauto].
         etrans; eauto. etrans; [|eauto].
         inv STEP_SRC; eauto. econs 2; eauto. econs; eauto.
